{-# OPTIONS --safe #-}

module Cubical.Tactics.PathSolver.MacroExamples where


open import Cubical.Foundations.Prelude
open import Cubical.Foundations.Structure
open import Cubical.Foundations.Function
open import Cubical.Foundations.Univalence
open import Cubical.Foundations.GroupoidLaws

open import Cubical.Relation.Nullary

open import Cubical.Data.Bool
open import Cubical.Data.Empty
open import Cubical.Data.Sum as ⊎
open import Cubical.Data.Maybe as Mb
open import Cubical.Data.List as L
open import Cubical.Data.Nat as ℕ
open import Cubical.Data.Sigma

open import Agda.Builtin.Nat using () renaming (_==_ to _=ℕ_ ; _<_ to _<ℕ_)
open import Agda.Builtin.String
open import Agda.Builtin.Char

open import Cubical.Data.Sigma.Base

open import Cubical.Reflection.Base renaming (v to 𝒗)
open import Cubical.Reflection.Sugar
import Agda.Builtin.Reflection as R
open import Cubical.Tactics.PathSolver.Reflection
open import Cubical.Tactics.Reflection

open import Cubical.Tactics.Reflection.Utilities

open import Cubical.Tactics.PathSolver.CongComp

open import Cubical.Tactics.Reflection.QuoteCubical

open import Cubical.Tactics.Reflection.Error
open import Cubical.Tactics.Reflection.Dimensions
open import Cubical.Tactics.Reflection.CuTerm
open import Cubical.Tactics.PathSolver.Reflection
open import Cubical.Tactics.Reflection.Variables
open import Cubical.Tactics.PathSolver.Degen
open import Cubical.Tactics.PathSolver.Path

open import Cubical.Tactics.PathSolver.Macro


private
  variable
    ℓ : Level
    A B : Type ℓ



module _ (SA : NPath 3 A) (f : A → B) where
  open NPath SA

  f[assoc] : cong f 𝑝₀ ∙ cong f 𝑝₁ ∙ cong f 𝑝₂ ≡ (cong f 𝑝₀ ∙ cong f 𝑝₁) ∙ cong f 𝑝₂
  f[assoc] i j = cong$ (f (assoc 𝑝₀ 𝑝₁ 𝑝₂ i j))


module _ (SA : NPath 6 A) (f : A → {A} → A → A) (g : A → A) (𝑝ₓ : g (NPath.𝑣₀ SA) ≡ g (NPath.𝑣₀ SA)) where
  open NPath SA

  p : f 𝑣₀ 𝑣₁ ≡ f 𝑣₃ 𝑣₆
  p i =  (f ((𝑝₀ ∙∙ 𝑝₁ ∙∙ 𝑝₂) i) {g ((𝑝₁ ∙' 𝑝₂) i)} ((𝑝₁ ∙∙ 𝑝₂ ∙∙ (𝑝₃ ∙∙ 𝑝₄ ∙∙ 𝑝₅)) i))

  
  _ :  (λ i → cong$ (p i))
        ≡
          (λ i → f (𝑝₀ i) {g (𝑝₁ i)} (𝑝₁ i))
      ∙∙  (λ i → f (𝑝₁ i) {g (𝑝₂ i)} (𝑝₂ i))
      ∙∙ ((λ i → f  𝑣₂    {g 𝑣₃}     (𝑝₃ i))
      ∙∙  (λ i → f (𝑝₂ i) {g 𝑣₃}     (𝑝₄ i))
      ∙∙   λ i → f  𝑣₃    {g 𝑣₃}     (𝑝₅ i))
  _ = refl

  cg² : ∀ {x y : A} → (x ≡ y) → g (g x) ≡ g (g y)
  cg² = congS (g ∘S g)

  cpf : Square (cong g 𝑝₀) (cong g (𝑝₀ ∙ 𝑝₁))
                refl          (cong g 𝑝₁)
  cpf i j = g (compPath-filler 𝑝₀ 𝑝₁ i j)

  cpf' : Square (cong g 𝑝₀) (cong g 𝑝₀ ∙ cong g 𝑝₁)
                 refl        (cong g 𝑝₁)
  cpf' i j = cong$ (cpf i j)


  cpf≡cpf' : Cube
              cpf cpf'
              _ _
              _ _
  cpf≡cpf' _ i j = cong! (cpf i j)



  cpf2 : Square (cong g (𝑝ₓ ∙ cong g (𝑝₀ ∙ 𝑝₁)))
               (cong g ((𝑝ₓ ∙ cong g (𝑝₀ ∙ 𝑝₁)) ∙ cong g (𝑝₂ ∙ 𝑝₃)))
               refl (cg² (𝑝₂ ∙ 𝑝₃))
  cpf2 i j = g (compPath-filler (𝑝ₓ ∙ cong g (𝑝₀ ∙ 𝑝₁)) (cong g (𝑝₂ ∙ 𝑝₃)) i j)

  cpf2' : Square
              (cong g 𝑝ₓ ∙ cg² 𝑝₀ ∙ cg² 𝑝₁)
               ((cong g 𝑝ₓ ∙ cg² 𝑝₀ ∙ cg² 𝑝₁) ∙ cg² 𝑝₂ ∙ cg² 𝑝₃)
                refl
               (cg² 𝑝₂ ∙ cg² 𝑝₃)
  cpf2' i j = cong$ (cpf2 i j)


  -- TODO : debug this
  -- cpf2≡cpf2' : Cube
  --             cpf2 cpf'
  --             _ _
  --             _ _
  -- cpf2≡cpf2' _ i j = cong! (cpf2 i j)



module _ (A : Type) (a : A) (p : a ≡ a) (s : Square p p p p)  where


 zz : Cube {A = A}
        _ _
        _ _
        _ _
 zz i j k = hcomp
              (λ { 𝒛₀ (i = i0) (j = i1) (k = i0) → a
                 ; 𝒛₀ (i = i1) → a
                 ; 𝒛₀ (k = i1) → hcomp
                                   (λ { 𝒛₁ (i = i0) → a
                                      ; 𝒛₁ (i = i1) → a
                                      ; 𝒛₁ (j = i0) → hcomp
                                                        (λ { 𝒛₂ (i = i0) → a
                                                           ; 𝒛₂ (i = i1) → a
                                                           ; 𝒛₂ (𝒛₀ = i0) → a
                                                           ; 𝒛₂ (𝒛₀ = i1) → a
                                                           ; 𝒛₂ (𝒛₁ = i0) → a
                                                           ; 𝒛₂ (𝒛₁ = i1) → a
                                                           })
                                                        a
                                      ; 𝒛₁ (j = i1) → a
                                      ; 𝒛₁ (𝒛₀ = i0) → a
                                      ; 𝒛₁ (𝒛₀ = i1) → a
                                      })
                                   a

                 ; 𝒛₀ (j = i0) → a
                 })
              (a)
